Progress. Nearly done.

extra/Secure/SecureEqProgInsens.v
@@ -1,5 +1,5 @@
 From Coinduction Require Import all.
-From Stdlib Require Import Morphisms.
+From Stdlib Require Import Morphisms Program.Basics.
 
 From ITree Require Import
      Axioms
@@ -29,67 +29,55 @@ Section SecureProgInsens.
   want it to be an equivalence
   *)
 
-  Variant pi_secure_eqitF (b1 b2 : bool) (l : L) vclo (sim : itree E R1 -> itree E R2 -> Prop) : itree' E R1 -> itree' E R2 -> Prop :=
+  Variant pi_secure_eqitF (b1 b2 : bool) (l : L) (sim : itree E R1 -> itree E R2 -> Prop) : itree' E R1 -> itree' E R2 -> Prop :=
 
     (* eqitF constructors *)
-    | pisecEqRet r1 r2 : RR r1 r2 -> pi_secure_eqitF b1 b2 l vclo sim (RetF r1) (RetF r2)
-    | pisecEqTau t1 t2 : sim t1 t2 -> pi_secure_eqitF b1 b2 l vclo sim (TauF t1) (TauF t2)
-    | pisecEqTauL t1 t2 (CHECK : b1) : sim t1 t2 -> pi_secure_eqitF b1 b2 l vclo sim (TauF t1) (observe t2)
-    | pisecEqTauR t1 t2 (CHECK : b2) : sim t1 t2 -> pi_secure_eqitF b1 b2 l vclo sim (observe t1) (TauF t2)
+    | pisecEqRet r1 r2 : RR r1 r2 -> pi_secure_eqitF b1 b2 l sim (RetF r1) (RetF r2)
+    | pisecEqTau t1 t2 : sim t1 t2 -> pi_secure_eqitF b1 b2 l sim (TauF t1) (TauF t2)
+    | pisecEqTauL t1 t2 (CHECK : b1) : sim t1 t2 -> pi_secure_eqitF b1 b2 l sim (TauF t1) (observe t2)
+    | pisecEqTauR t1 t2 (CHECK : b2) : sim t1 t2 -> pi_secure_eqitF b1 b2 l sim (observe t1) (TauF t2)
     (* info_flow protecting coinductive constructors *)
     | piEqVisPriv {A} (e : E A) k1 k2 (SECCHECK : leq (priv A e) l) :
-        ((forall a, vclo sim (k1 a) (k2 a) : Prop)) -> pi_secure_eqitF b1 b2 l vclo sim (VisF e k1) (VisF e k2)
+        ((forall a, sim (k1 a) (k2 a) : Prop)) -> pi_secure_eqitF b1 b2 l sim (VisF e k1) (VisF e k2)
     | piEqVisUnPrivTauLCo {A} (e : E A) k1 t2 (SECCHECK : ~ leq (priv A e) l) :
-        (forall a, vclo sim (k1 a) t2) -> pi_secure_eqitF b1 b2 l vclo sim (VisF e k1) (TauF t2)
+        (forall a, sim (k1 a) t2) -> pi_secure_eqitF b1 b2 l sim (VisF e k1) (TauF t2)
     | piEqVisUnPrivTauRCo {A} (e : E A) t1 k2 (SECCHECK : ~ leq (priv A e) l) :
-        (forall a, vclo sim t1 (k2 a)) -> pi_secure_eqitF b1 b2 l vclo sim (TauF t1) (VisF e k2)
+        (forall a, sim t1 (k2 a)) -> pi_secure_eqitF b1 b2 l sim (TauF t1) (VisF e k2)
     | piEqVisUnPrivVisCo {A B} (e1 : E A) (e2 : E B) k1 k2 (SECCHECK1 : ~ leq (priv A e1) l) (SECCHECK2 : ~ leq (priv B e2) l)
         :
-        (forall a b, vclo sim (k1 a) (k2 b)) -> pi_secure_eqitF b1 b2 l vclo sim (VisF e1 k1) (VisF e2 k2)
+        (forall a b, sim (k1 a) (k2 b)) -> pi_secure_eqitF b1 b2 l sim (VisF e1 k1) (VisF e2 k2)
     (* info_flow protecting inductive constructors *)
     | piEqVisUnPrivLInd {A} (e : E A) k1 t2 (CHECK : b1) (SECCHECK : ~ leq (priv A e) l) :
-        (forall a, vclo sim (k1 a) t2 ) ->
-        pi_secure_eqitF b1 b2 l vclo sim (VisF e k1) (observe t2)
+        (forall a, sim (k1 a) t2 ) ->
+        pi_secure_eqitF b1 b2 l sim (VisF e k1) (observe t2)
     | piEqVisUnPrivRInd {A} (e : E A) t1 k2 (CHECK : b2) (SECCHECK : ~ leq (priv A e) l) :
-        (forall a, vclo sim t1 (k2 a) ) ->
-        pi_secure_eqitF b1 b2 l vclo sim (observe t1) (VisF e k2)
+        (forall a, sim t1 (k2 a) ) ->
+        pi_secure_eqitF b1 b2 l sim (observe t1) (VisF e k2)
   .
 
   Hint Constructors pi_secure_eqitF : itree.
 
-  Definition pi_secure_eqit_ (b1 b2 : bool) (l : L) vclo (sim : itree E R1 -> itree E R2 -> Prop) : itree E R1 -> itree E R2 -> Prop :=
-    fun t1 t2 => pi_secure_eqitF b1 b2 l vclo sim (observe t1) (observe t2).
+  Definition pi_secure_eqit_ (b1 b2 : bool) (l : L) (sim : itree E R1 -> itree E R2 -> Prop) : itree E R1 -> itree E R2 -> Prop :=
+    fun t1 t2 => pi_secure_eqitF b1 b2 l sim (observe t1) (observe t2).
 
   Hint Unfold pi_secure_eqit_ : itree.
 
-  Lemma pi_secure_eqitF_mono b1 b2 l x0 x1 vclo vclo' sim sim'
-        (IN: pi_secure_eqitF b1 b2 l vclo sim x0 x1)
-        (MON: monotone2 vclo)
-        (LEc: vclo <3= vclo')
-        (LE: sim <2= sim'):
-    pi_secure_eqitF b1 b2 l vclo' sim' x0 x1.
+  Lemma pi_secure_eqitF_mono b1 b2 l :
+    Proper (respectful Coinduction.lattice.leq Coinduction.lattice.leq)
+      (pi_secure_eqit_ b1 b2 l).
   Proof.
-    intros. induction IN; eauto with itree.
+    intros!. red; red in H0.
+    induction H0; try solve [constructor; intros; eauto with itree; now apply H].
   Qed.
 
-  Lemma pi_secure_eqit_mono b1 b2 l vclo (MON: monotone2 vclo) : monotone2 (pi_secure_eqit_ b1 b2 l vclo).
-  Proof.
-    do 2 red. intros; eapply pi_secure_eqitF_mono; eauto with itree.
-  Qed.
+  Definition pi_secure_eqit_mon b1 b2 l := Build_mon (pi_secure_eqitF_mono b1 b2 l).
 
-  Hint Resolve pi_secure_eqit_mono : paco.
-
-  Definition pi_eqit_secure b1 b2 l := paco2 (pi_secure_eqit_ b1 b2 l id) bot2.
-
-  (* want and eqitC_secure which could help prove some interesting stuff
-
-   *)
-
+  Definition pi_eqit_secure b1 b2 l := gfp (pi_secure_eqit_mon b1 b2 l).
 
 End SecureProgInsens.
 
-#[export] Hint Resolve pi_secure_eqit_mono : paco.
 #[export] Hint Constructors pi_secure_eqitF : itree.
+#[global] Hint Constructors pi_secure_eqitF : itree.
 
 Ltac unpriv_pi := try apply piEqVisUnPrivVisCo;
                   try apply piEqVisUnPrivTauLCo;
@@ -102,126 +90,116 @@ Ltac contra_size :=
   match goal with
   | [ Hemp : empty ?A, Hne : nonempty ?A |- _ ] => inv Hemp; inv Hne; contradiction end.
 
+#[local] Ltac taul := apply pisecEqTauL; [auto|].
+#[local] Ltac taur := apply pisecEqTauR; [auto|].
 
 Lemma eqit_secure_imp_pi_eqit_scure b1 b2 E R1 R2 RR Label priv l : forall (t1 : itree E R1) (t2 : itree E R2),
     eqit_secure Label priv RR b1 b2 l t1 t2 -> pi_eqit_secure Label priv RR b1 b2 l t1 t2.
 Proof.
-  coinduction c CIH. intros t1 t2 Hps. step. step in Hps. red in Hps.
-  hinduction Hps before r; intros.
+  icoinduction c CIH. intros t1 t2 Hps. step in Hps.
+  hinduction Hps before c; intros.
   - constructor; auto with itree.
-  - constructor. right.  eauto with itree.
-  - rewrite itree_eta'. constructor; auto with itree. eapply CIH.  step. apply Hps.
-  - rewrite itree_eta' at 1. constructor; auto with itree. eapply CIH.  step. apply Hps.
-  -  constructor; auto with itree. right. eapply CIH; eauto with itree. apply H.
-  -  unpriv_pi. right. eapply CIH; apply H.
-  -  unpriv_pi. right. eapply CIH; apply H.
-  -  unpriv_pi. right. eapply CIH; apply H.
-  -  unpriv_pi. eapply CIH.  step. apply H.
-  -  unpriv_pi. eapply CIH.  step. apply H.
-  - unpriv_pi. inv SIZECHECK. contradiction.
-  - unpriv_pi. inv SIZECHECK. contradiction.
-  - unpriv_pi. inv SIZECHECK. contradiction.
-  - unpriv_pi. inv SIZECHECK. contradiction.
+  - constructor. apply CIH. apply H.
+  - rewrite itree_eta'. constructor; auto with itree. eapply CIH. step. apply Hps.
+  - rewrite itree_eta' at 1. constructor; auto with itree. eapply CIH. step. apply Hps.
+  - constructor; auto with itree. intros. apply CIH. apply H.
+  - unpriv_pi. eapply CIH; apply H.
+  - unpriv_pi. eapply CIH; apply H.
+  - unpriv_pi. eapply CIH; apply H.
+  - unpriv_pi. eapply CIH. step. apply H.
+  - unpriv_pi. eapply CIH. step. apply H.
+  - unpriv_pi; inv SIZECHECK; contradiction.
+  - unpriv_pi; inv SIZECHECK; contradiction.
+  - unpriv_pi; inv SIZECHECK; contradiction.
+  - unpriv_pi; inv SIZECHECK; contradiction.
 Qed.
 
 
 Lemma pi_eqit_secure_sym b1 b2 E R1 R2 RR Label priv l : forall (t1 : itree E R1) (t2 : itree E R2),
     pi_eqit_secure Label priv RR b1 b2 l t1 t2 -> pi_eqit_secure Label priv (flip RR) b2 b1 l t2 t1.
 Proof.
-  coinduction c CIH. intros t1 t2 Hsec.
-  step in Hsec. step. red in Hsec. red. inversion Hsec;  eauto;
-  try (unpriv_pi; right; eapply CIH; apply H1; fail).
-  constructor; auto. right. eapply CIH; apply H1.
+  icoinduction c CIH. intros t1 t2 Hsec. step in Hsec.
+  hinduction Hsec before c; intros; eauto with itree;
+  try (unpriv_pi; apply CIH; apply H; fail).
+  constructor; auto. intros. apply CIH. apply H.
 Qed.
 
 
-Lemma pi_secure_eqit_mon : forall E (b1 b2 b3 b4 : bool) R1 R2 RR1 RR2 Label priv l
+Lemma pi_secure_eqit_mono : forall E (b1 b2 b3 b4 : bool) R1 R2 RR1 RR2 Label priv l
       (t1 : itree E R1) (t2 : itree E R2),
-    (b1 -> b3) -> (b2 -> b4) -> (RR1 <2= RR2) ->
+    (b1 -> b3) -> (b2 -> b4) -> (RR1 <= RR2) ->
     pi_eqit_secure Label priv RR1 b1 b2 l t1 t2 -> pi_eqit_secure Label priv RR2 b3 b4 l t1 t2.
 Proof.
   intros. generalize dependent t2. revert t1. coinduction c CIH.
-  intros t1 t2 Ht12. pstep. red.
-  step in Ht12. red in Ht12.
-  hinduction Ht12 before r; intros; eauto; 
-  try (unpriv_pi; right; apply CIH; try red; eauto; fail);
-  constructor; auto. right.  eauto. apply CIH; apply H2.
+  intros t1 t2 Ht12. icbn.
+  step in Ht12.
+  hinduction Ht12 before l; intros;
+  try (unpriv_pi; apply CIH; try red; eauto; fail);
+  eauto with itree.
+  - constructor; auto. now apply H2.
+  - constructor; intros; eauto. eapply CIH. apply H.
 Qed.
 
 
 Lemma pi_eqit_secure_spin b E R1 R2 (RR : R1 -> R2 -> Prop) Label priv l : forall (t1 : itree E R1),
     pi_eqit_secure Label priv RR b true l t1 (ITree.spin).
 Proof.
-  coinduction c CIH. intros. step. cbn. constructor; auto.
+  icoinduction c CIH. intros. cbn. constructor; auto.
 Qed.
 
 Lemma pi_eqit_secure_private_halt b E R1 R2 (RR : R1 -> R2 -> Prop) Label priv l A (e : E A) k:
   empty A -> ~ leq (priv A e) l -> forall (t1 : itree E R1),
     pi_eqit_secure Label priv RR b true l t1 (Vis e k).
 Proof.
-  intros HA t1. step. cbn. intros. unpriv_pi. inv HA; contradiction.
+  intros HA Hleq t1. step. cbn. unpriv_pi. inv HA; contradiction.
 Qed.
 
 Lemma pi_eqit_secure_mixed_trans_aux1:
   forall (E : Type -> Type) (R1 : Type) (b2 : bool) (R2 : Type) (RR1 : R1 -> R2 -> Prop)
     (Label : Preorder) (priv : forall A : Type, E A -> L) (l : L) t1 t2,
-    paco2 (pi_secure_eqit_ Label priv RR1 true b2 l id) bot2 t1 (Tau t2)  ->
+    pi_eqit_secure Label priv RR1 true b2 l t1 (Tau t2)  ->
     pi_eqit_secure Label priv RR1 true b2 l t1 t2.
 Proof.
   intros E R1 b2 R2 RR1 Label priv l. coinduction c CIH.
-  intros t1 t2 Htau. step in Htau. red in Htau.
-  step. cbn in *. inv Htau;  eauto.
-  - constructor; auto. left. eapply paco2_mon; eauto. intros; contradiction.
-  - constructor; auto. right. eapply CIH; eauto. step. rewrite <- H0.
-    cbn. pstep_reverse.
-  - pstep_reverse. eapply paco2_mon; eauto. intros; contradiction.
-  - unpriv_pi. left.  eapply paco2_mon; eauto. intros; contradiction.
-  - unpriv_pi. eapply CIH.  step. rewrite <- H0.
-    cbn. pstep_reverse.
+  intros t1 t2 Htau. step in Htau.
+  icbn. cbn in *.
+  inv Htau; eauto with itree.
+  - constructor; auto. apply (gfp_chain c). apply H1.
+  - constructor; auto. apply CIH. step. rewrite <- H0. step in H1. apply H1.
+  - apply (gfp_bchain c). apply H1.
+  - unpriv_pi. apply (gfp_chain c). apply H1.
+  - unpriv_pi. apply CIH. step. rewrite <- H0. specialize (H1 a). step in H1. apply H1.
 Qed.
 
 Lemma pi_eqit_secure_mixed_trans b1 b2 E R1 R2 R3 (RR1 : R1 -> R2 -> Prop) (RR2 : R2 -> R3 -> Prop)
       Label priv l : forall (t1 : itree E R1) t2 t3,
-    pi_eqit_secure Label priv RR1 b1 b2 l t1 t2 -> eqit RR2 b1 b2 t2 t3 ->
+    pi_eqit_secure Label priv RR1 b1 b2 l t1 t2 -> eqit b1 b2 RR2 t2 t3 ->
     pi_eqit_secure Label priv (rcompose RR1 RR2) b1 b2 l t1 t3.
 Proof.
-  coinduction c CIH. intros t1 t2 t3 Hsec Heq. step in Heq.
-  red in Heq. step in Hsec. red in Hsec. step. red.
-  hinduction Heq before r; intros; 
-  - inv Hsec; eauto with itree; unpriv_pi; 
-    + rewrite itree_eta'. constructor; auto with itree. right. eapply CIH; eauto.
-      step. rewrite H0. constructor. auto.
-    + rewrite itree_eta'. unpriv_pi. right. eapply CIH; eauto.
-      apply H1. step. rewrite H0. constructor; auto.
-  - inv Hsec;  eauto with itree.
-    + constructor. right. eapply CIH; eauto with itree.
-      step. rewrite H0. constructor; auto. pstep_reverse.
-    + unpriv_pi. right. eapply CIH; eauto. apply H1.
-    + rewrite itree_eta'. unpriv_pi. right. eapply CIH; eauto.
-      inv CHECK. apply pi_eqit_secure_mixed_trans_aux1.
-      step. rewrite <- H0. cbn. pstep_reverse.
+  coinduction c CIH. intros t1 t2 t3 Hsec Heq.
+  step in Heq. step in Hsec. icbn. cbn in *.
+  hinduction Heq before c; intros.
+  - inv Hsec; eauto with itree; unpriv_pi.
+    + rewrite itree_eta'. constructor; auto with itree. eapply CIH; eauto. step. rewrite H0. constructor. auto.
+    + rewrite itree_eta'. unpriv_pi. eapply CIH; eauto. apply H1. step. rewrite H0. constructor; auto.
+  - inv Hsec; eauto with itree.
+    + constructor. eapply CIH; eauto with itree. step. rewrite H0. constructor; auto. now step in REL.
+    + unpriv_pi. eapply CIH; eauto. apply H1.
+    + unpriv_pi. eapply CIH. apply H1. step. rewrite H0. apply EqTauL; auto. now step in REL.
   - inv Hsec.
-    +  rewrite itree_eta'. constructor; auto. right. eapply CIH; eauto.
-      step. rewrite H0. constructor. left. auto.
-    + ddestruction. subst. constructor; auto with itree. right.
-       eapply CIH; eauto with itree. apply H1.
-    + ddestruction. subst. unpriv_pi. right. 
-      eapply CIH; eauto with itree. apply H1.
-    + ddestruction. subst. unpriv_pi. right. 
-      eapply CIH; eauto with itree. apply H1.
-    +  remember (VisF e k2) as ovis. rewrite itree_eta'.
-      unpriv_pi. rewrite Heqovis. right. eapply CIH; eauto with itree. apply H1.
-      step. rewrite H0. constructor. left. auto.
-    + ddestruction. subst. unpriv_pi. right. eapply CIH; eauto with itree.  apply H1.
-  - eapply IHHeq; eauto. clear IHHeq. inv Hsec; 
+    + rewrite itree_eta'. constructor; auto. eapply CIH; eauto. step. rewrite H0. apply EqVis. apply REL.
+    + ddestruction. subst. constructor; auto with itree. intros a. eapply CIH. apply H1. apply REL.
+    + ddestruction. subst. unpriv_pi. eapply CIH. apply H1. apply REL.
+    + ddestruction. subst. unpriv_pi. eapply CIH. apply H1. apply REL.
+    + remember (VisF e k2) as ovis. rewrite itree_eta'. unpriv_pi. rewrite Heqovis. eapply CIH. apply H1. step. rewrite H0. apply EqVis. apply REL.
+    + ddestruction. subst. unpriv_pi. eapply CIH. apply H1. apply REL.
+  - eapply IHHeq; eauto. clear IHHeq. inv Hsec.
     + constructor; auto.
-    + constructor; auto. left. apply pi_eqit_secure_mixed_trans_aux1. step. red.
-      rewrite <- H0. cbn. pstep_reverse.
-    + pstep_reverse.
+    + inv CHECK. constructor; auto. apply pi_eqit_secure_mixed_trans_aux1. step. rewrite <- H0. now step in H1.
+    + now step in H1.
     + unpriv_pi.
-    + unpriv_pi. left. apply pi_eqit_secure_mixed_trans_aux1. step. red.
-      rewrite <- H0. cbn. pstep_reverse.
-  - constructor; auto. left. step. eapply IHHeq; eauto.
+    + inv CHECK0. unpriv_pi. apply pi_eqit_secure_mixed_trans_aux1. step. rewrite <- H0. specialize (H1 a). step in H1. apply H1.
+  - constructor; auto. step. eapply IHHeq; eauto.
 Qed.
 
 Lemma pi_eqit_secure_RR_imp b1 b2 E R1 R2 (RR1 : R1 -> R2 -> Prop ) (RR2 : R1 -> R2 -> Prop)
@@ -230,121 +208,55 @@ Lemma pi_eqit_secure_RR_imp b1 b2 E R1 R2 (RR1 : R1 -> R2 -> Prop ) (RR2 : R1 ->
       pi_eqit_secure Label priv RR1 b1 b2 l t1 t2 ->
       pi_eqit_secure Label priv RR2 b1 b2 l t1 t2.
 Proof.
-  intro Himp. coinduction c CIH.
-  intros. step. step in H0. red in H0.
-  inv H0; eauto;
-  try (constructor; auto;  eauto; fail);
-  try ( constructor; auto; right; eapply CIH; eauto; try apply H2; fail).
+  intros Himp.
+  icoinduction c CIH. intros t1 t2 Ht12. step in Ht12.
+  hinduction Ht12 before c; intros; eauto with itree;
+  try ( constructor; auto; intros; eapply CIH; eauto; fail);
+  try ( unpriv_pi; intros; eapply CIH; eauto; apply H; fail).
+  constructor; auto. intros. eapply CIH. apply H.
 Qed.
 
-Lemma pi_eqit_secureC_wcompat_id :  forall b1 b2 E R1 R2 (RR : R1 -> R2 -> Prop )
-      Label priv l
-, wcompatible2 (@pi_secure_eqit_ E R1 R2 Label priv RR b1 b2 l id)
-                                         (eqitC RR b1 b2) .
+Ltac inv_eq_itree := 
+  repeat match goal with 
+  | [ H : eqitF _ false false _ (RetF _) _ |- _ ] => inv H
+  | [ H : eqitF _ false false _ _ (RetF _) |- _ ] => inv H
+  | [ H : eqitF _ false false _ (TauF _) _ |- _ ] => inv H
+  | [ H : eqitF _ false false _ _ (TauF _) |- _ ] => inv H
+  | [ H : eqitF _ false false _ (VisF _ _) _ |- _ ] => inv H
+  | [ H : eqitF _ false false _ _ (VisF _ _) |- _ ] => inv H
+  end. 
+(* Chain-level congruence: rewriting under [eq_itree eq] on either side of a
+   chain element.  This replaces the paco-style [pi_eqit_secureC_wcompat_id]
+   (weak compatibility of the [eqitC] up-to-eutt closure).  Template:
+   [euttge_proper_secureC] in [SecureEqEuttHalt.v]. *)
+#[global] Instance pi_eqit_secure_proper_secureC {E R1 R2} b1 b2 Label priv (RR : R1 -> R2 -> Prop) l
+  (c : Chain (pi_secure_eqit_mon Label priv RR b1 b2 l)) :
+  Proper (eq_itree (E := E) eq ==> eq_itree eq ==> flip impl) (elem c).
 Proof.
-  econstructor. pmonauto_itree.
-  intros. destruct PR.
-  step in EQVl. step in EQVr. unfold_eqit. red in REL. red.
-  hinduction REL before r; intros; clear t1' t2'.
-  - genobs_clear t1 ot1. genobs_clear t2 ot2.
-    remember (RetF r1) as x.
-    hinduction EQVl before r; intros; inv Heqx; eauto.
-    + remember (RetF r3) as y.
-      hinduction EQVr before r; intros; inv Heqy; eauto with itree.
-      rewrite itree_eta' at 1. constructor; eauto with itree. gstep. red.
-      eapply IHEQVr; eauto.
-    + rewrite itree_eta'. constructor; auto. cbn. gstep. cbn.
-      eauto.
-  - remember (TauF t1) as y.
-    hinduction EQVl before r; intros; inv Heqy; subst; eauto.
-    + remember (TauF t2) as x.
-      hinduction EQVr before r; intros; inv Heqx; subst; eauto.
-       constructor. gclo. econstructor; eauto with paco.
-      
-      remember (TauF m1) as ot1. rewrite itree_eta' at 1.
-      constructor; auto. rewrite Heqot1. gstep. cbn. eauto.
-    + constructor; auto. gstep. eapply IHEQVl; eauto.
-  - inv EQVl. 
-    + constructor; auto. gclo. econstructor; eauto with paco itree.
-    + constructor; auto. gclo. econstructor; eauto with paco itree.
-      apply eqit_inv_Tau_r. step. auto.
-  - inv EQVr.
-    + constructor; auto. gclo. econstructor; eauto with paco itree.
-    + constructor; auto. gclo. econstructor; eauto with paco itree.
-      apply eqit_inv_Tau_r. step. auto.
-  - remember (VisF e k1) as x.
-    hinduction EQVl before r; intros; inv Heqx; eauto.
-    + ddestruction. subst. remember (VisF e0 k3) as y.
-      hinduction EQVr before r; intros; inv Heqy; eauto.
-      * ddestruction. subst. constructor; auto.
-        intros. apply gpaco2_clo.  econstructor; eauto with itree. apply H.
-      *  remember (VisF e0 k1) as ovis. rewrite itree_eta' at 1.
-        constructor; auto. rewrite Heqovis. gstep. eapply IHEQVr; eauto with itree.
-    + constructor; auto. gstep. eapply IHEQVl; eauto.
-  - remember (VisF e k1) as x.
-    hinduction EQVl before r; intros; inv Heqx; subst; eauto.
-    + ddestruction. subst.  remember (TauF t2) as y.
-      hinduction EQVr before r; intros; inv Heqy; subst;  eauto.
-      * unpriv_pi. gclo. econstructor; cycle -1; eauto with paco itree. gfinal. left. apply H.
-      * remember (VisF e0 k1) as ovis. rewrite itree_eta' at 1. constructor; auto.
-        rewrite Heqovis. gstep. eapply IHEQVr; eauto.
-    + constructor; auto. gstep. eapply IHEQVl; eauto.
-  - remember (TauF t1) as x.
-    hinduction EQVl before r; intros; inv Heqx; subst; eauto.
-    + remember (VisF e k2) as y.
-      hinduction EQVr before r; intros; inv Heqy; subst; eauto.
-      * ddestruction. subst.
-         unpriv_pi. gclo. econstructor; cycle -1; eauto with paco itree.
-        gfinal. left. apply H.
-      * remember (TauF m1) as otm1. rewrite itree_eta' at 1. constructor; auto.
-        gstep. rewrite Heqotm1. red. eapply IHEQVr; eauto.
-   + constructor; auto. gstep. eapply IHEQVl; eauto.
-  - remember (VisF e1 k1) as x.
-    hinduction EQVl before r; intros; inv Heqx; subst; eauto.
-    + ddestruction. subst. remember (VisF e2 k3) as y.
-      hinduction EQVr before r; intros; inv Heqy; subst; eauto.
-      * ddestruction. subst. unpriv_pi. gclo. 
-        econstructor; eauto with paco itree. gfinal. left. apply H.
-      * remember (VisF e1 k1) as ovis. rewrite itree_eta' at 1.
-        constructor; auto. rewrite Heqovis. gstep. eapply IHEQVr; eauto.
-    + remember (VisF e2 k2) as x.
-      hinduction EQVr before r; intros; inv Heqx; subst; eauto.
-      * ddestruction. subst.  unpriv_pi.
-         gclo. eapply eqit_trans_clo_intro with (t1' := Vis e1 k0); eauto with paco itree.
-         gstep. cbn. unpriv_pi. gfinal. left. apply H.
-       * remember (TauF t3) as ott3. rewrite itree_eta' at 1. constructor; auto.
-         rewrite Heqott3. gstep. eapply IHEQVr; eauto.
-  - remember (VisF e k1) as x.
-    hinduction EQVl before r; intros; inv Heqx; eauto.
-    + ddestruction. subst.  unpriv_pi.
-      gclo. econstructor; eauto with paco itree. gfinal. left. apply H.
-    + constructor; auto. gstep. eapply IHEQVl; eauto.
-  - remember (VisF e k2) as x.
-    hinduction EQVr before r; intros; inv Heqx; eauto.
-    + ddestruction. subst.  unpriv_pi.
-      gclo. econstructor; eauto with paco itree. gfinal. left. apply H.
-    + constructor; auto. gstep. eapply IHEQVr; eauto.
-Qed.
+  do 5 red. tower induction. clear c. intros c CIH t1 t2 H12 t3 t4 H34 Hpi.
+  icbn; icbn in Hpi. step in H12; step in H34. 
+  induction Hpi; inv_eq_itree.
+  (* ret and coinductive cases are simple *)
+  1,2: eauto with itree. 
+  - taul. eapply CIH. apply REL. step; apply H34. assumption. 
+  - taur. eapply CIH. step; apply H12. apply REL. assumption. 
+  - ddestruction. evis.  
+  - ddestruction. unpriv_pi. eapply CIH. apply REL0. apply REL. apply H. 
+  - ddestruction. unpriv_pi. eapply CIH. apply REL. apply REL0. apply H.
+  - ddestruction. unpriv_pi. eapply CIH. apply REL0. apply REL. apply H.
+  - ddestruction. unpriv_pi. eapply CIH. apply REL. step; apply H34. apply H. 
+  - ddestruction. unpriv_pi. eapply CIH. step; apply H12. apply REL. apply H.
+Qed. 
 
-#[export] Hint Resolve pi_eqit_secureC_wcompat_id : paco.
-
-Global Instance geuttgen_cong_secure_eqit {E} {Label priv l} {R1 R2 : Type} {RR1 : R1 -> R1 -> Prop}
-    {RR2 : R2 -> R2 -> Prop} {RS : R1 -> R2 -> Prop} (b1 b2 : bool) {r rg} :
-    (forall (x x' : R1) (y : R2), (RR1 x x' : Prop) -> (RS x' y : Prop) -> RS x y) ->
-    (forall (x : R1) (y y' : R2), (RR2 y y' : Prop) -> RS x y' -> RS x y) ->
-    Proper (@eq_itree E R1 R1 RR1 ==> eq_itree RR2 ==> flip impl)
-           (gpaco2 (pi_secure_eqit_ Label priv RS b1 b2 l id) (eqitC RS b1 b2) r rg ).
+(* ... lift to the gfp via [chain_gfp]: this is the [Proper] instance the
+   downstream chain-style [rewrite]s depend on, replacing the paco
+   [geuttgen_cong_*] gpaco instances. *)
+#[global] Instance pi_eqit_secure_eutt_proper {E} {Label priv l} {R1 R2 : Type} {RS : R1 -> R2 -> Prop} (b1 b2 : bool) :
+   Proper (@eq_itree E R1 R1 eq ==> eq_itree eq ==> flip impl)
+          (pi_eqit_secure Label priv RS b1 b2 l).
 Proof.
-  repeat intro. gclo. econstructor; eauto with itree.
-  - eapply eqit_mon, H1; eauto; discriminate.
-  - eapply eqit_mon, H2; eauto; discriminate.
-Qed.
-
-Global Instance geuttgen_cong_eq_secure_eqit {E} {Label priv l} {R1 R2 : Type} {RS : R1 -> R2 -> Prop} (b1 b2 : bool) {r rg} :
-    Proper (@eq_itree E R1 R1 eq ==> eq_itree eq ==> flip impl)
-           (gpaco2 (pi_secure_eqit_ Label priv RS b1 b2 l id) (eqitC RS b1 b2) r rg ).
-Proof.
-  eapply geuttgen_cong_secure_eqit; eauto; intros; subst; auto.
+  eapply pi_eqit_secure_proper_secureC with
+    (c := chain_gfp (pi_secure_eqit_mon Label priv RS b1 b2 l)).
 Qed.
 
 Global Instance pi_eqit_secure_eq_itree_proper {E} {Label priv l} {R1 R2 : Type} {RS : R1 -> R2 -> Prop} (b1 b2 : bool) :
@@ -353,21 +265,16 @@ Global Instance pi_eqit_secure_eq_itree_proper {E} {Label priv l} {R1 R2 : Type}
 Proof.
   intros t1 t2 Ht12 t3 t4 Ht34. intros Hsec.
   apply pi_eqit_secure_RR_imp with (RR1 := rcompose RS eq).
-  { intros. inv H. auto. }
-  eapply pi_eqit_secure_mixed_trans. 2: { symmetry in Ht34. apply Ht34. }
+  intros r0 r3 Hr; inv Hr; auto.
+  eapply pi_eqit_secure_mixed_trans; cycle 1.
+  symmetry in Ht34. apply Ht34.
   apply pi_eqit_secure_sym in Hsec. apply pi_eqit_secure_sym.
   symmetry in Ht12.
   apply pi_eqit_secure_RR_imp with (RR1 := rcompose (flip RS) eq).
-  { intros. inv H. auto. }
+  intros r0 r3 Hr; inv Hr; auto.
   eapply pi_eqit_secure_mixed_trans; eauto.
 Qed.
 
-Global Instance pi_eqit_secure_eutt_proper {E} {Label priv l} {R1 R2 : Type} {RS : R1 -> R2 -> Prop} (b1 b2 : bool) :
-   Proper (@eq_itree E R1 R1 eq ==> eq_itree eq ==> flip impl)
-          (pi_eqit_secure Label priv RS b1 b2 l).
-Proof.
-  repeat intro. ginit. rewrite H, H0. gfinal. eauto.
-Qed.
 
 Lemma pi_eqit_secure_ret E Label priv l b1 b2 R1 R2 (RR : R1 -> R2 -> Prop) r1 r2 :
   RR r1 r2 -> @pi_eqit_secure E R1 R2 Label priv RR b1 b2 l (Ret r1) (Ret r2).
@@ -381,48 +288,41 @@ Lemma pi_eqit_secure_bind E Label priv l b1 b2 R1 R2 S1 S2 (RR : R1 -> R2 -> Pro
     pi_eqit_secure Label priv RR b1 b2 l t1 t2 ->
     pi_eqit_secure Label priv RS b1 b2 l (ITree.bind t1 k1) (ITree.bind t2 k2).
 Proof.
-  ginit. gcofix CIH. intros. sinv H1.
-  - apply simpobs in H. apply simpobs in H2. rewrite H. rewrite H2.
-    repeat rewrite bind_ret_l. gfinal. right. eapply paco2_mon; try apply H0; auto.
-    intros; contradiction.
-  - apply simpobs in H. apply simpobs in H2. rewrite H. rewrite H2.
-    repeat rewrite bind_tau. gstep. constructor. gfinal. left. eapply CIH; eauto.
-  - apply simpobs in H. apply simpobs in H2.  rewrite H2. rewrite H. rewrite bind_tau.
-    gstep. constructor; auto. gfinal. left. eapply CIH; eauto.
-    step. cbn. pstep_reverse.
-  - apply simpobs in H. apply simpobs in H2.  rewrite H2. rewrite H. rewrite bind_tau.
-    gstep. constructor; auto. gfinal. left. eapply CIH; eauto.
-    step. cbn. pstep_reverse.
-  - apply simpobs in H. apply simpobs in H2. rewrite H. rewrite H2.
-    repeat rewrite bind_vis. gstep. constructor; auto.
-    gfinal. left. eapply CIH; eauto. apply H3.
-  - apply simpobs in H. apply simpobs in H2. rewrite H. rewrite H2.
-    rewrite bind_vis. rewrite bind_tau. gstep. cbn. unpriv_pi.
-    gfinal. left. eapply CIH; eauto. apply H3.
-  - apply simpobs in H. apply simpobs in H2. rewrite H. rewrite H2.
-    rewrite bind_vis. rewrite bind_tau. gstep. cbn. unpriv_pi.
-    gfinal. left. eapply CIH; eauto. apply H3.
-  - apply simpobs in H. apply simpobs in H2. rewrite H. rewrite H2.
-    repeat rewrite bind_vis. gstep. cbn. unpriv_pi.
-    gfinal. left. eapply CIH; eauto. apply H3.
-  - apply simpobs in H. apply simpobs in H2. rewrite H. rewrite H2.
-    rewrite bind_vis. gstep. unpriv_pi.
-    gfinal. left. eapply CIH; eauto. step. cbn. pstep_reverse.
-  - apply simpobs in H. apply simpobs in H2. rewrite H. rewrite H2.
-    rewrite bind_vis. gstep. unpriv_pi.
-    gfinal. left. eapply CIH; eauto. step. cbn. pstep_reverse.
-Qed.
+  icoinduction c CIH. intros ?? Hk1k2 Ht1t2.
+  step in Ht1t2.
+  genobs t1 Hot1. 
+  genobs t2 Hot2. 
+  hinduction Ht1t2 before c; intros.
+  - rewrite 2observe_bind. simpobs. step. apply Hk1k2. apply H. 
+  - rewrite 2observe_bind. simpobs. etau. 
+  - rewrite observe_bind. simpobs. taul.  
+    eapply CIH; intros; auto. step. simpobs. now unstep. 
+  - rewrite (observe_bind t3). simpobs. taur.
+    eapply CIH; intros; auto. step. simpobs. now unstep.
+  - rewrite 2observe_bind. simpobs. constructor; auto. intros. 
+    eapply CIH; intros; auto. step. simpobs. now unstep.
+  - rewrite 2observe_bind. simpobs. unpriv_pi. 
+    eapply CIH; intros; auto. step. simpobs. now unstep.
+  - rewrite 2observe_bind. simpobs. unpriv_pi. 
+    eapply CIH; intros; auto. step. simpobs. now unstep.
+  - rewrite 2observe_bind. simpobs. unpriv_pi. 
+    eapply CIH; intros; auto. step. simpobs. now unstep.
+  -  rewrite observe_bind. simpobs. unpriv_pi. 
+    eapply CIH; intros; auto. step. simpobs. now unstep.
+  - rewrite (observe_bind t2). simpobs. unpriv_pi. 
+    eapply CIH; intros; auto. step. simpobs. now unstep.
+Qed. 
 
 Lemma pi_eqit_secure_iter_bind_aux:
   forall (E : Type -> Type) (B2 B1 A1 A2 : Type) (RA : A1 -> A2 -> Prop)
     (RB : B1 -> B2 -> Prop) (b1 b2 : bool) (Label : Preorder)
     (priv : forall A : Type, E A -> L) (l : L) (body1 : A1 -> itree E (A1 + B1))
-    (body2 : A2 -> itree E (A2 + B2)) (r : itree E B1 -> itree E B2 -> Prop),
-    (forall (a1 : A1) (a2 : A2), RA a1 a2 -> r (ITree.iter body1 a1) (ITree.iter body2 a2)) ->
+    (body2 : A2 -> itree E (A2 + B2))
+    (c : Chain (pi_secure_eqit_mon Label priv RB b1 b2 l)),
+    (forall (a1 : A1) (a2 : A2), RA a1 a2 -> elem c (ITree.iter body1 a1) (ITree.iter body2 a2)) ->
     forall (t1 : itree E (A1 + B1)) (t2 : itree E (A2 + B2)),
-      paco2 (pi_secure_eqit_ Label priv (HeterogeneousRelations.sum_rel RA RB) b1 b2 l id) bot2 t1
-            t2 ->
-      gpaco2 (pi_secure_eqit_ Label priv RB b1 b2 l id) (eqitC RB b1 b2) r r
+      pi_eqit_secure Label priv (HeterogeneousRelations.sum_rel RA RB) b1 b2 l t1 t2 ->
+      elem c
              (ITree.bind t1
                          (fun lr : A1 + B1 =>
                             match lr with
@@ -436,33 +336,31 @@ Lemma pi_eqit_secure_iter_bind_aux:
                             | inr r0 => Ret r0
                             end)).
 Proof.
-  intros E B2 B1 A1 A2 RA RB b1 b2 Label priv l body1 body2 r CIH t1 t2 H2.
-  generalize dependent t2. revert t1. gcofix CIH'. intros t1 t2 Ht12.
-  sinv Ht12; apply simpobs in H; apply simpobs in H0.
-  - rewrite H, H0. repeat rewrite bind_ret_l. inv H1.
-    + gstep. constructor. gfinal. left. apply CIH'0. eapply CIH; eauto.
-    + gstep. constructor; auto.
-  - rewrite H, H0. repeat rewrite bind_tau. gstep. constructor.
-    gfinal. left. eapply CIH'; eauto.
-  - rewrite H. rewrite <- itree_eta in H0. rewrite H0. rewrite bind_tau. gstep.
-    constructor; auto. gfinal.
-    left. eapply CIH'; eauto.
-  - rewrite H0. rewrite <- itree_eta in H. rewrite H. rewrite bind_tau. gstep.
-    constructor; auto. gfinal.
-    left. eapply CIH'; eauto.
-  - rewrite H, H0. repeat rewrite bind_vis. gstep. constructor; auto.
-    intros. gfinal. left. eauto.
-  - rewrite H, H0. rewrite bind_vis, bind_tau.  gstep. unpriv_pi; auto.
-    intros. gfinal. left. eauto.
-  - rewrite H, H0. rewrite bind_vis, bind_tau.  gstep. unpriv_pi; auto.
-    intros. gfinal. left. eauto.
-  - rewrite H, H0. repeat rewrite bind_vis. gstep. unpriv_pi.
-    gfinal. left. eauto.
-  - rewrite H. rewrite <- itree_eta in H0. rewrite H0. rewrite bind_vis.
-    gstep. unpriv_pi. gfinal. left. eauto.
-  - rewrite H0. rewrite <- itree_eta in H. rewrite H. rewrite bind_vis.
-    gstep. unpriv_pi. gfinal. left. eauto.
-Qed.
+  intros E B2 B1 A1 A2 RA RB b1 b2 Label priv l body1 body2 c. 
+  tower induction. clear c; intros c CIH Hbody t1 t2 Ht12. step in Ht12. 
+  icbn. genobs t1 ot1. genobs t2 ot2.
+  hinduction Ht12 before E; intros. 
+  #[local] Ltac by_coinduction CIH := 
+  eapply CIH; intros; 
+  try solve [now step; simpobs; unstep]; 
+  match goal with
+  | |- elem _ _ _ => Utils.step 
+  end; auto. 
+  (* QUESTION: why does 'now step; apply Hbody' instead of auto fail? *)
+  #[local] Ltac pi_solve CIH := constructor; auto; intros; by_coinduction CIH.
+  - unfold observe; cbn; simpobs. inv H; cbn; eauto with itree.
+    constructor. now step; apply Hbody. 
+  - unfold observe; cbn; simpobs. pi_solve CIH.
+  - unfold observe at 1; cbn; simpobs. pi_solve CIH.
+  - unfold observe at 2; cbn; simpobs. pi_solve CIH.
+  - unfold observe; cbn; simpobs. pi_solve CIH.
+  - unfold observe; cbn; simpobs. pi_solve CIH.
+  - unfold observe; cbn; simpobs. pi_solve CIH.
+  - unfold observe; cbn; simpobs. pi_solve CIH.
+  - unfold observe at 1; cbn; simpobs. pi_solve CIH.
+  - unfold observe at 2; cbn; simpobs. pi_solve CIH.
+Qed. 
+
 
 Lemma secure_eqit_iter E A1 A2 B1 B2 (RA : A1 -> A2 -> Prop) (RB : B1 -> B2 -> Prop)
                            b1 b2 Label priv l
@@ -471,34 +369,5 @@ Lemma secure_eqit_iter E A1 A2 B1 B2 (RA : A1 -> A2 -> Prop) (RB : B1 -> B2 -> P
                            forall (a1 : A1) (a2 : A2), RA a1 a2 ->
     pi_eqit_secure Label priv RB b1 b2 l (ITree.iter body1 a1) (ITree.iter body2 a2).
 Proof.
-  intro Hbody. ginit. gcofix CIH. intros. rewrite unfold_iter. rewrite unfold_iter.
-  apply Hbody in H0. sinv H0; apply simpobs in H; apply simpobs in H1.
-  - rewrite H. rewrite H1. repeat rewrite bind_ret_l. inv H2.
-    + gstep. constructor. gfinal. left. eapply CIH; eauto.
-    + gstep. constructor; auto.
-  - rewrite H. rewrite H1. repeat rewrite bind_tau. gstep.
-    constructor. eapply pi_eqit_secure_iter_bind_aux; eauto.
-  - rewrite H. rewrite bind_tau. gstep. constructor; auto.
-    eapply pi_eqit_secure_iter_bind_aux; eauto.
-    assert (t1 ≈ body1 a1).
-    { rewrite H. rewrite tau_eutt. reflexivity. }
-    inv CHECK. rewrite <- itree_eta in H1. rewrite H1. auto.
-  - rewrite H1. rewrite bind_tau. gstep. constructor; auto.
-    eapply pi_eqit_secure_iter_bind_aux; eauto. rewrite H.
-    rewrite <- itree_eta. apply H2.
-  - rewrite H, H1. repeat rewrite bind_vis. gstep. constructor; auto.
-    intros. red.
-    eapply pi_eqit_secure_iter_bind_aux; eauto.
-  - rewrite H, H1. rewrite bind_vis, bind_tau. gstep. unpriv_pi.
-    eapply pi_eqit_secure_iter_bind_aux; eauto.
-  - rewrite H, H1. rewrite bind_vis, bind_tau. gstep. unpriv_pi.
-    eapply pi_eqit_secure_iter_bind_aux; eauto.
-  - rewrite H, H1. repeat rewrite bind_vis. gstep. unpriv_pi.
-    eapply pi_eqit_secure_iter_bind_aux; eauto.
-  - rewrite H. rewrite bind_vis. gstep. unpriv_pi.
-    eapply pi_eqit_secure_iter_bind_aux; eauto.
-    rewrite H1. rewrite <- itree_eta. apply H2.
-  - rewrite H1. rewrite bind_vis. gstep. unpriv_pi. red.
-    rewrite H. rewrite <- itree_eta.
-    eapply pi_eqit_secure_iter_bind_aux; eauto.
-Qed.
+  (* TODO(paco->coinduction): fill in (template: secure_eqit_iter in SecureEqBind.v). *)
+Admitted.
